src/heaplang/adequacy.v
@@ -1,19 +1,161 @@
-From iris.itree Require Import wpi.
+From iris.itree Require Import wpi ub.
 From iris.itree.threadpool Require Import trace.
-From iris.itree.heaplang Require Import lang.
 From iris Require Import invariants ghost_map.
 From iris.proofmode Require Import proofmode.
 From ITree Require Import ITree Recursion RecursionFacts InterpFacts Eqit.
 From iris.program_logic Require Import language.
-
+From iris.itree.threadpool Require Import handler.
+From iris.itree.heaplang Require Import lang.
 Context {Σ} `{!invGS_gen hlc Σ} `{!heaplangHGS Σ}.
+
+Lemma compile_Fork {R} e (k : val → itree heaplangE R) :
+  (v ← compile_expr (Fork e) ; k v)%itree ≈ vis EFork (λ thread,
+    match thread with
+    | CurrentThread => k (LitV LitUnit)
+    | NewThread =>
+        v ← compile_expr e;
+        kill_thread
+    end
+  )%itree.
+Proof.
+  rewrite /compile_expr !rec_as_interp interp_bind.
+  setoid_rewrite interp_trigger. simpl.
+  rewrite -bind_trigger bind_bind. f_equiv. intros [|].
+  - rewrite interp_ret bind_ret_l //.
+  - rewrite rec_as_interp interp_bind bind_bind. f_equiv. intros v.
+    rewrite /kill_thread. rewrite interp_vis /= bind_vis bind_vis.
+    apply eqit_VisF. intros [].
+Qed.
+
+Lemma trace_base_Fork {R} tid (tp : list (itree heaplangE R)) tr e k :
+  tp !! tid = Some (v ← compile_expr (Fork e) ; k v)%itree →
+  is_ctrace tr tid (<[tid := k (LitV LitUnit)]>tp ++ [(compile_expr e ;; kill_thread)%itree]) →
+  is_ctrace (CTFork (compile_expr e ;; kill_thread) tr) tid tp.
+Proof.
+  intros Htp Htr. eapply is_ctrace_insert; first done; first apply compile_Fork; eauto.
+  eexists. split. { rewrite list_lookup_insert //. by apply lookup_lt_is_Some_1. }
+  constructor.
+  rewrite /compile_expr rec_as_interp //. rewrite list_insert_insert.
+  destruct Htr as (t'&Ht'&Htr).
+  simpl in Ht'.
+  rewrite lookup_app_l in Ht'; last rewrite insert_length -lookup_lt_is_Some //.
+  rewrite list_lookup_insert in Ht'; last by apply lookup_lt_is_Some_1.
+  by injection Ht' as <-.
+Qed.
+
+Lemma base_BinOp op v1 v2 v3 :
+  bin_op_eval op v1 v2 = Some v3 →
+  compile_expr (BinOp op (Val v1) (Val v2)) ≈ Ret v3.
+Proof.
+  intros Hop.
+  rewrite /compile_expr !rec_as_interp interp_bind interp_ret bind_ret_l /=
+    interp_bind interp_ret bind_ret_l interp_bind interp_ret bind_ret_l
+    interp_bind interp_ret bind_ret_l Hop interp_ret //.
+Qed.
+
+Lemma base_Beta f_ x_ e v :
+  compile_expr (App (Val (RecV f_ x_ e)) (Val v))
+  ≈ let e' := (subst' x_ v (subst' f_ (RecV f_ x_ e) e))
+     in yield_if_not_val e' ;; compile_expr e'.
+Proof.
+  rewrite /compile_expr !rec_as_interp interp_bind interp_ret bind_ret_l /=
+    interp_bind interp_ret bind_ret_l interp_bind interp_ret bind_ret_l
+    interp_bind interp_ret bind_ret_l interp_bind /yield_if_not_val.
+  destruct (is_value _) eqn:Heq.
+  - rewrite interp_ret !bind_ret_l rec_as_interp.
+    setoid_rewrite interp_trigger. rewrite /= rec_as_interp //.
+  - setoid_rewrite interp_trigger. f_equiv; first done. by intros _.
+Qed.
+
+Lemma step_in_thread {R} e1 σ1 κs e2 σ2 efs tr tid tid' tp (k : val → itree heaplangE R) :
+  base_step e1 σ1 κs e2 σ2 efs →
+  is_ctrace tr tid' (<[tid:=(v ← compile_expr e2 ; yield_if_not_val e2 ;; k v)%itree]>tp
+                    ++ map (λ e, compile_expr e ;; kill_thread)%itree efs) →
+  tp !! tid = Some (v ← compile_expr e1 ; yield_if_not_val e1 ;; k v)%itree →
+  ∃ tr', is_postfix tr tr' ∧ is_ctrace tr' tid tp.
+Proof.
+  intros Hbase Htr Htp.
+  inversion Hbase; subst; simpl in Htr; rewrite ?app_nil_r in Htr.
+  - admit.
+  - admit.
+  - admit.
+  - admit.
+  - pose (e' := subst' x v2 (subst' f (RecV f x e0) e0)).
+    exists (CTYield tid' tr). split; first repeat constructor.
+    destruct (is_value e') eqn:Hval.
+    * eapply is_ctrace_insert; first done.
+      { simpl. rewrite base_Beta. simpl.
+        rewrite /yield_if_not_val. rewrite /e' in Hval. rewrite Hval. rewrite bind_ret_l.
+        reflexivity. }
+      rewrite /e' in Hval. apply is_value_val in Hval as [v Heq].
+      rewrite Heq in Htr. rewrite Heq.
+      rewrite compile_expr_val. rewrite compile_expr_val in Htr.
+      simpl in Htr.
+      rewrite bind_ret_l. rewrite !bind_ret_l in Htr.
+      apply ctrace_yield with (t := k v).
+      { rewrite list_lookup_insert //. by apply lookup_lt_is_Some. }
+      by rewrite list_insert_insert.
+    * eapply is_ctrace_insert; first done.
+      { simpl. rewrite base_Beta. simpl. rewrite /yield_if_not_val. rewrite /e' in Hval.
+        rewrite Hval. reflexivity. }
+      rewrite /e' in Hval. rewrite /yield_if_not_val in Htr. rewrite Hval in Htr.
+      rewrite bind_bind.
+      apply ctrace_yield with (t := (v ← compile_expr e'; trigger EYield ;; k v)%itree).
+      { rewrite list_lookup_insert //. by apply lookup_lt_is_Some. }
+      by rewrite list_insert_insert.
+  - admit.
+  - exists (CTYield tid' tr). split; first repeat constructor.
+    rewrite compile_expr_val !bind_ret_l in Htr.
+    eapply is_ctrace_insert with (t' := (trigger EYield ;; k v')%itree); first done.
+    { rewrite base_BinOp // bind_ret_l  //. }
+    eapply ctrace_yield. { rewrite list_lookup_insert //. by apply lookup_lt_is_Some. }
+    by rewrite list_insert_insert.
+  - admit.
+  - admit.
+  - admit.
+  - admit.
+  - admit.
+  - admit.
+  - (* AllocN *) admit.
+  - admit.
+  - admit.
+  - admit.
+  - admit.
+  - admit.
+  - admit.
+  - exists (CTFork (compile_expr e ;; kill_thread) (CTYield tid' tr)).
+    split; first repeat constructor.
+    rewrite compile_expr_val !bind_ret_l in Htr.
+    eapply trace_base_Fork; first apply Htp.
+    eapply ctrace_yield.
+    { rewrite lookup_app_l; last rewrite insert_length -lookup_lt_is_Some //.
+      rewrite list_lookup_insert //. by apply lookup_lt_is_Some. }
+    rewrite insert_app_l; last rewrite insert_length -lookup_lt_is_Some //.
+    rewrite list_insert_insert //.
+Admitted.
+
+Lemma base_step_in_thread_completed {R} e1 σ1 κs e2 σ2 efs tr tid tid' (tp : list (itree heaplangE R)) :
+  base_step e1 σ1 κs e2 σ2 efs →
+  is_value e2 →
+  is_ctrace tr tid' (delete tid tp ++ map (λ e, compile_expr e ;; kill_thread)%itree efs) →
+  tp !! tid = Some (compile_expr e1 ;; kill_thread)%itree →
+  ∃ tr', is_postfix tr tr' ∧ is_ctrace tr' tid tp.
+Admitted.
+
+Lemma base_step_in_thread_not_completed {R} e1 σ1 κs e2 σ2 efs tr tid tid' (tp : list (itree heaplangE R)) :
+  base_step e1 σ1 κs e2 σ2 efs →
+  ~is_value e2 →
+  is_ctrace tr tid' (<[tid:=(compile_expr e2 ;; kill_thread)%itree]>tp ++ map (λ e, compile_expr e ;; kill_thread)%itree efs) →
+  tp !! tid = Some (compile_expr e1 ;; kill_thread)%itree →
+  ∃ tr', is_postfix tr tr' ∧ is_ctrace tr' tid tp.
+Admitted.
 
 (* TODO: The idea is to add that if [tp'] has nowhere to step then [tr] ends in
 *        UB, and if [tp'] returns a value, then so does [tr]. *)
 Lemma has_trace n tp σ tp' σ' κ :
   nsteps n (tp, σ) κ (tp', σ') →
   length tp > 0 →
-  ∃ tr i, is_ctrace tr i (map compile_expr tp).
+  ∃ tr i, is_ctrace tr i (map compile_expr (filter unevaluated tp)).
 Proof.
   revert tp σ tp' σ' κ. induction n; intros tp σ tp' σ' κ Hstep Hne.
   { exists CTCut, 0. destruct tp as [|t tp]. { simpl in Hne. lia. }
